proofs for straightline pass (with admits for some depth stuff that should be unneeded soon)

src/Experiments/SimplyTypedArithmetic.v
@@ -7958,7 +7958,7 @@ Module Straightline.
         Definition dummy t : expr t := Scalar (dummy_scalar t).
       End with_ident.
 
-      Definition scalar_of_uncurried_ident {s d} (idc : ident.ident s d)
+      Definition of_uncurried_scalar_ident {s d} (idc : ident.ident s d)
         : scalar s -> option (scalar d) :=
         match idc in ident.ident s d return scalar (ident:=ident.ident) s -> option (scalar d) with
         | ident.Z.cast r => fun args => Some (Cast r args)
@@ -7973,18 +7973,18 @@ Module Straightline.
         | _ => fun _ => None
         end.
 
-      Fixpoint scalar_of_uncurried {t} (e : uexpr t) : option (scalar t) :=
+      Fixpoint of_uncurried_scalar {t} (e : uexpr t) : option (scalar t) :=
           match e in Uncurried.expr.expr t return option (scalar t) with
           | expr.Var t v as e => Some (Var t v)
           | expr.TT as e => Some TT
           | expr.Pair A B a b
-            => match scalar_of_uncurried a, scalar_of_uncurried b with
+            => match of_uncurried_scalar a, of_uncurried_scalar b with
                | Some x, Some y => Some (Pair x y)
                | _, _ => None
                end
           | expr.AppIdent _ _ idc args
-            => match scalar_of_uncurried args with
-               | Some x => scalar_of_uncurried_ident idc x
+            => match of_uncurried_scalar args with
+               | Some x => of_uncurried_scalar_ident idc x
                | None => None
                end
           | _ => None
@@ -8027,7 +8027,7 @@ Module Straightline.
         | Some (r, x, e) =>
           match invert_AppIdent x with
           | Some (existT s idc_x') =>
-            match scalar_of_uncurried (snd idc_x') with
+            match of_uncurried_scalar (snd idc_x') with
             | Some x'' =>
               match invert_Abs e with
               | Some k => Some (existT _ s (r, fst idc_x', x'', k))
@@ -8066,7 +8066,7 @@ Module Straightline.
           fun (args : uexpr _) default =>
             match invert_AppIdent args with
             | Some (existT s idc_x') =>
-              match scalar_of_uncurried (snd idc_x') with
+              match of_uncurried_scalar (snd idc_x') with
               | Some x'' =>
                 @mk_LetInAppIdent s type.Z type.Z default r (fst idc_x') x'' (fun y => Scalar (Var _ y))
               | None => default
@@ -8077,7 +8077,7 @@ Module Straightline.
           fun (args : uexpr _) default =>
             match invert_AppIdent args with
             | Some (existT s idc_x') =>
-              match scalar_of_uncurried (snd idc_x') with
+              match of_uncurried_scalar (snd idc_x') with
               | Some x'' =>
                 @mk_LetInAppIdent s (type.Z*type.Z) (type.Z*type.Z) default r (fst idc_x') x'' (fun y => Scalar (Var _ y))
               | None => default
@@ -8091,14 +8091,20 @@ Module Straightline.
                  (of_uncurried : forall t, uexpr t -> expr t)
                  : expr t -> expr t :=
         match e in Uncurried.expr.expr t return expr t -> expr t with
-         | AppIdent s d idc args => of_uncurried_ident of_uncurried idc args
+        | AppIdent s d idc args =>
+          fun default =>
+            of_uncurried_ident of_uncurried idc args
+                               (match of_uncurried_scalar (AppIdent idc args) with
+                                | Some s => Scalar s
+                                | None => default
+                                end)
          | _ as e  =>
            (fun default =>
-              match scalar_of_uncurried e with
+              match of_uncurried_scalar e with
               | Some s => Scalar s
               | None => default
               end)
-         end.
+        end.
 
       (* TODO : uses fuel; ideally want a cleaner termination proof *)
       Fixpoint of_uncurried (fuel : nat) {t} (e : uexpr t)
@@ -8107,24 +8113,285 @@ Module Straightline.
         | S fuel' => of_uncurried_step e (@of_uncurried fuel') (dummy t)
         | O => dummy t
         end.
-
     End with_var.
-  End expr.
 
-  Fixpoint depth {var t} (dummy_var : forall t, var t) (e : @Uncurried.expr.expr ident.ident var t) : nat :=
-    match e with
-    | Uncurried.expr.Var _ _ => O
-    | Uncurried.expr.TT => O
-    | Uncurried.expr.AppIdent _ _ idc args => S (depth dummy_var args)
-    | Uncurried.expr.App _ _ f x => S (Nat.max (depth dummy_var f) (depth dummy_var x))
-    | Uncurried.expr.Pair _ _ x y => S (Nat.max (depth dummy_var x) (depth dummy_var y))
-    | Uncurried.expr.Abs _ _ f => S (depth dummy_var (f (dummy_var _)))
-    end.
+    Section depth.
+      Context (var : type -> Type) (dummy_var : forall t, var t).
+      Fixpoint depth {t} (e : @Uncurried.expr.expr ident var t) : nat :=
+        match e with
+        | Uncurried.expr.Var _ _ => 1
+        | Uncurried.expr.TT => 1
+        | Uncurried.expr.AppIdent _ _ idc args => S (depth args)
+        | Uncurried.expr.App _ _ f x => S (Nat.max (depth f) (depth x))
+        | Uncurried.expr.Pair _ _ x y => S (Nat.max (depth x) (depth y))
+        | Uncurried.expr.Abs _ _ f => S (depth (f (dummy_var _)))
+        end.
+
+      Definition Expr_depth {t} (e : Expr t) : nat := depth (e _).
+    End depth.
+
+    Section interp.
+      Local Notation scalar := (@scalar type.interp default.ident).
+      Local Notation expr := (@expr type.interp default.ident).
+
+      Definition interp_cast (r : zrange) (x : Z) : Z := ident.cast ident.cast_outside_of_range r x.
+      
+      Fixpoint interp_scalar {t} (s : scalar t) : type.interp t :=
+        match s with
+        | Var t v => v
+        | TT => tt
+        | Nil _ => []
+        | Pair _ _ x y => (interp_scalar x, interp_scalar y)
+        | Cast r x => interp_cast r (interp_scalar x)
+        | Cast2 r x =>
+          let '(a,b) := interp_scalar x in (interp_cast (fst r) a, interp_cast (snd r) b)
+        | Fst _ _ p => fst (interp_scalar p)
+        | Snd _ _ p => snd (interp_scalar p)
+        | Shiftr n x => Z.shiftr (interp_scalar x) n
+        | Shiftl n x => Z.shiftl (interp_scalar x) n
+        | Land n x => Z.land (interp_scalar x) n
+        | CC_m n x => Z.cc_m n (interp_scalar x)
+        | Primitive _ x => x
+        end.
+      
+      Fixpoint interp {t} (e : expr t) : type.interp t :=
+        match e with
+        | Scalar _ s => interp_scalar s
+        | LetInAppIdentZ _ _ r idc x f =>
+          interp (f (interp_cast r (ident.interp idc (interp_scalar x))))
+        | LetInAppIdentZZ _ _ (r1,r2) idc x f =>
+          let '(a,b) := ident.interp idc (interp_scalar x) in
+          interp (f (interp_cast r1 a, interp_cast r2 b))
+        end.
+
+      Inductive ok_scalar_ident : forall {s d}, ident.ident s d -> Prop :=
+      | ok_si_cast : forall r, ok_scalar_ident (ident.Z.cast r)
+      | ok_si_cast2 : forall r, ok_scalar_ident (ident.Z.cast2 r)
+      | ok_si_fst : forall A B, ok_scalar_ident (@ident.fst A B)
+      | ok_si_snd : forall A B, ok_scalar_ident (@ident.snd A B)
+      | ok_si_shiftr : forall n, ok_scalar_ident (@ident.Z.shiftr n)
+      | ok_si_shiftl : forall n, ok_scalar_ident (@ident.Z.shiftl n)
+      | ok_si_land : forall n, ok_scalar_ident (@ident.Z.land n)
+      | ok_si_cc_m : forall n, ok_scalar_ident (@ident.Z.cc_m_concrete n)
+      | ok_prim : forall p x, ok_scalar_ident (@ident.primitive p x)
+      .
+
+      Inductive ok_scalar: forall {t}, @Uncurried.expr.expr ident type.interp t -> Prop :=
+      | ok_Var : forall t v, @ok_scalar t (Uncurried.expr.Var v)
+      | ok_TT : ok_scalar Uncurried.expr.TT
+      | ok_AppIdent :
+          forall s d idc args,
+            ok_scalar args ->
+            @ok_scalar_ident s d idc ->
+            ok_scalar (AppIdent idc args)
+      | ok_Pair :
+          forall A B a b,
+            @ok_scalar A a ->
+            @ok_scalar B b ->
+            ok_scalar (Uncurried.expr.Pair a b)
+      .
+
+      Inductive ok_expr : forall {t}, Uncurried.expr.expr t -> Prop :=
+      | ok_LetInAppIdentZ :
+          forall tC r s (idc : ident s type.Z) x k,
+            ok_scalar x -> (forall y, @ok_expr tC (k y)) ->
+            @ok_expr tC (AppIdent (@ident.Let_In _ tC) (Uncurried.expr.Pair (AppIdent (ident.Z.cast r) (AppIdent idc x)) (Abs k)))
+      | ok_LetInAppIdentZZ :
+          forall tC r s (idc : ident s (type.prod type.Z type.Z)) x k,
+            ok_scalar x -> (forall y, @ok_expr tC (k y)) ->
+            @ok_expr tC (AppIdent (@ident.Let_In _ tC) (Uncurried.expr.Pair (AppIdent (ident.Z.cast2 r) (AppIdent idc x)) (Abs k)))
+      | ok_scalar_cast :
+          forall r s (idc : ident s  _) x,
+            ok_scalar x ->
+            ok_scalar_ident idc ->
+            @ok_expr type.Z (AppIdent (ident.Z.cast r) (AppIdent idc x))
+      | ok_scalar_cast2 :
+          forall r s (idc : ident s _) x,
+            ok_scalar x ->
+            ok_scalar_ident idc ->
+            @ok_expr (type.prod type.Z type.Z) (AppIdent (ident.Z.cast2 r) (AppIdent idc x))
+      | ok_scalar_nocast :
+          forall t x, @ok_scalar t x -> @ok_expr t x
+      .
+
+      Lemma interp_cast_correct {t} r (idc : ident t type.Z) x :
+        interp_cast r (ident.interp idc (expr.interp (@ident.interp) x))
+        = expr.interp (@ident.interp) (AppIdent (ident.Z.cast r) (AppIdent idc x)).
+      Proof. reflexivity. Qed.
+
+      Lemma interp_cast2_correct {t} r1 r2 (idc : ident t (type.prod type.Z type.Z)) x :
+        (interp_cast r1 (fst (ident.interp idc (expr.interp (@ident.interp) x))),
+         interp_cast r2 (snd (ident.interp idc (expr.interp (@ident.interp) x))))
+        = expr.interp (@ident.interp) (AppIdent (ident.Z.cast2 (r1, r2)) (AppIdent idc x)).
+      Proof. cbn; break_match; reflexivity. Qed.
+
+      Definition primitive_eq_dec (a b : type.primitive) : {a = b} + {a <> b}.
+      Proof. destruct a,b; auto; right; congruence. Defined.
+      Fixpoint type_eq_dec (a b : type) : {a = b} + {a <> b}.
+      Proof.
+        destruct a, b; try solve [right; congruence]; [ | | | ].
+        { destruct (primitive_eq_dec p p0); subst; [left | right]; congruence. }
+        { destruct (type_eq_dec a1 b1); destruct (type_eq_dec a2 b2); subst; try solve [right; congruence].
+          left; congruence. }
+        { destruct (type_eq_dec a1 b1); destruct (type_eq_dec a2 b2); subst; try solve [right; congruence].
+          left; congruence. }
+        { destruct (type_eq_dec a b); [left | right]; congruence. }
+      Defined.
+
+      Ltac invert H :=
+        inversion H; subst;
+        repeat match goal with
+               | H : existT _ _ _ = existT _ _ _ |- _ => apply (Eqdep_dec.inj_pair2_eq_dec _ type_eq_dec) in H; subst
+               end.
+
+      Ltac invert_ok_expr :=
+        match goal with H : ok_expr _ |- _ => invert H end.
+      Ltac invert_ok_scalar :=
+        match goal with H : ok_scalar _ |- _ => invert H end.
+      Ltac invert_ok_scalar_ident :=
+        match goal with H : ok_scalar_ident _ |- _ => invert H end.
+      Ltac simpl_inversions :=
+        cbn [invert_LetInAppIdent invert_LetInCast invert_Pair invert_cast invert_AppIdent invert_Abs].
+
+      Lemma invert_AppIdent_correct {d} (e : @Uncurried.expr.expr ident type.interp d) x p :
+        invert_AppIdent e = Some (existT (fun s : type => (ident s d * default.expr s)%type) x p) ->
+        e = AppIdent (fst p) (snd p).
+      Proof.
+        cbv [invert_AppIdent].
+        break_match; try discriminate.
+        intro H; invert H. reflexivity.
+      Qed.
+
+      Lemma depth_positive {var t} dummy_var (e : Uncurried.expr.expr t) : 0 < depth var dummy_var e.
+      Proof. destruct e; cbn [depth]; rewrite Nat2Z.inj_succ; omega. Qed.
+
+      Lemma of_uncurried_scalar_ident_correct {s d} (idc : ident s d) args args':
+        ok_scalar_ident idc ->
+        of_uncurried_scalar args = Some args' ->
+        interp_scalar args' = expr.interp (@ident.interp) args ->
+        exists s,
+          of_uncurried_scalar_ident idc args' = Some s
+          /\ interp_scalar s = expr.interp (@ident.interp) (AppIdent idc args).
+      Proof.
+        destruct 1; intros;
+          repeat match goal with
+                 | _ => eexists; split; [ reflexivity | cbn [interp_scalar] ]
+                 | H : interp_scalar _ = _ |- _ => rewrite H
+                 | _ => reflexivity
+                 end.
+        { cbn; break_match; reflexivity. }
+        { cbn; break_match; reflexivity. }
+      Qed.
+
+      Lemma of_uncurried_scalar_correct {t} (e : Uncurried.expr.expr t) :
+        ok_scalar e ->
+        exists s,
+          of_uncurried_scalar e = Some s
+          /\ interp_scalar s = expr.interp (@ident.interp) e.
+      Proof.
+        induction 1; cbn [of_uncurried_scalar]; intros;
+          repeat match goal with
+                 | IH : exists _, _ /\ _ |- _ => destruct IH as [? [? ?] ]
+                 | H : of_uncurried_scalar _ = _ |- _ => rewrite H
+                 | _ => apply of_uncurried_scalar_ident_correct; solve [auto]
+                 | _ => eexists; tauto
+                 end; [ ].
+        eexists; split; [ reflexivity | ].
+        cbn [interp_scalar expr.interp].
+        congruence.
+      Qed.
+
+      Ltac rewrite_ok_scalar :=
+        match goal with H : ok_scalar _ |- _ =>
+                        let P := fresh in destruct (of_uncurried_scalar_correct _ H) as [? [P ?] ]; rewrite P in *
+        end;
+        repeat match goal with
+               | H : Some _ = Some _ |- _ => inversion H; progress subst
+               | _ => progress break_match;
+                      match goal with | H: Some _ = Some _ |- _ => inversion H; progress subst end
+               end.
+      
+      Lemma of_uncurried_correct dummy_arrow fuel dummy_var :
+        forall {t} (e : @Uncurried.expr.expr ident type.interp t),
+        (depth _ dummy_var e <= fuel)%nat ->
+        ok_expr e ->
+        expr.interp (@ident.interp) e = interp (@of_uncurried _ dummy_arrow fuel _ e).
+      Proof.
+        induction fuel; intros; [ pose proof (depth_positive dummy_var e); omega | ].
+        destruct e; cbn [depth of_uncurried expr.interp interp]; intros; invert_ok_expr;
+          repeat match goal with
+                 | |- context [of_uncurried_scalar _ ] => progress rewrite_ok_scalar
+                 | _ => progress (cbn [of_uncurried_step of_uncurried_ident fst snd mk_LetInAppIdent expr.interp interp depth] in * )
+                 | _ => progress simpl_inversions
+                 | _ => congruence
+                 end; [ | | | | ].
+        {
+          match goal with H : interp_scalar _ = _ |- _ => rewrite H end.
+          rewrite <-IHfuel; rewrite interp_cast_correct.
+          { reflexivity. }
+          { cbn [depth] in *.
+            (* here we have to reason about the depth calculation for arrows; this will probably be unnecessary with new compilers setup *)
+            admit. }
+          { auto. } }
+        {
+          match goal with H : interp_scalar _ = _ |- _ => rewrite H end.
+          break_match.
+          match goal with H : ?p = (?x, ?y) |- _ =>
+                          replace x with (fst p) by (rewrite H; reflexivity);
+                          replace y with (snd p) by (rewrite H; reflexivity)
+          end.
+          rewrite <-IHfuel. rewrite interp_cast2_correct.
+          { cbn; break_match; reflexivity. }
+          { cbn [depth] in *.
+            (* here we have to reason about the depth calculation for arrows; this will probably be unnecessary with new compilers setup *)
+            admit. }
+          { auto. } }
+        {
+          match goal with H : interp_scalar _ = _ |- _ => rewrite H end.
+          rewrite interp_cast_correct.
+          reflexivity. }
+        {
+          match goal with H : interp_scalar _ = _ |- _ => rewrite H end.
+          break_match.
+          match goal with H : ?p = (?x, ?y) |- _ =>
+                          replace x with (fst p) by (rewrite H; reflexivity);
+                          replace y with (snd p) by (rewrite H; reflexivity)
+          end.
+          rewrite interp_cast2_correct.
+          cbn; break_match; reflexivity. }
+        { invert_ok_scalar.
+          rewrite <-H2.
+          invert_ok_scalar_ident; try reflexivity.
+          { match goal with H : context [of_uncurried_scalar _ = Some _ ] |- _ => cbn in H end.
+            rewrite_ok_scalar.
+            cbn [of_uncurried_ident].
+            cbn [interp_scalar].
+            cbn.
+            break_match; cbn; auto.
+            match goal with H : _ |- _ => apply invert_AppIdent_correct in H end.
+            subst.
+            invert_ok_scalar.
+            rewrite_ok_scalar.
+            repeat match goal with H : interp_scalar _ = _ |- _ => rewrite H end.
+            reflexivity. }
+          { match goal with H : context [of_uncurried_scalar _ = Some _ ] |- _ => cbn in H end.
+            rewrite_ok_scalar.
+            cbn [of_uncurried_ident].
+            break_match; cbn; auto.
+            match goal with H : _ |- _ => apply invert_AppIdent_correct in H end.
+            subst.
+            invert_ok_scalar.
+            rewrite_ok_scalar.
+            repeat match goal with H : interp_scalar _ = _ |- _ => rewrite H end.
+            destruct r; reflexivity. }
+        Admitted.
+    End interp.
+  End expr.
 
   Definition of_Expr {s d} (e : Expr (s->d)) (var : type -> Type) (x:var s) dummy_arrow: expr.expr d
     :=
       match invert_Abs (e var) with
-      | Some f => expr.of_uncurried (dummy_arrow:=dummy_arrow) (depth (var:=fun _ => unit) (fun _ => tt) (e (fun _ => unit))) (f x)
+      | Some f => expr.of_uncurried (dummy_arrow:=dummy_arrow) (expr.depth (fun _ => unit) (fun _ => tt) (e (fun _ => unit))) (f x)
       | None => expr.dummy (dummy_arrow:=dummy_arrow) d
       end.
 
